updates

Veritas.Verifier.Thread.fst
@@ -4,7 +4,7 @@ let rec lemma_verifiable_implies_prefix_verifiable_aux
   (tl:verifiable_log) (i:nat{i <= length tl}):
   Lemma (requires (True))
         (ensures (verifiable (prefix tl i)))
-        (decreases (length tl)) = 
+        (decreases (length tl)) =
   let n = length tl in
   if i = n then ()
   else lemma_verifiable_implies_prefix_verifiable_aux (prefix tl (n - 1)) i
@@ -24,15 +24,15 @@ let rec lemma_clock_monotonic_aux (tl:verifiable_log) (i:idx tl):
     let tl' = prefix tl (n - 1) in
     lemma_clock_monotonic_aux tl' i
 
-let lemma_clock_monotonic (tl: verifiable_log) (i:idx tl) (j:idx tl{j >= i}): 
-  Lemma (clock tl i `ts_leq` clock tl j) = 
+let lemma_clock_monotonic (tl: verifiable_log) (i:idx tl) (j:idx tl{j >= i}):
+  Lemma (clock tl i `ts_leq` clock tl j) =
   let tlj = prefix tl (j + 1) in
   lemma_clock_monotonic_aux tlj i
 
 let rec lemma_thread_id_state_aux (tl: verifiable_log):
   Lemma (requires True)
-        (ensures (V.thread_id_of (verify tl) = thread_id_of tl)) 
-        (decreases (length tl)) = 
+        (ensures (V.thread_id_of (verify tl) = thread_id_of tl))
+        (decreases (length tl)) =
   let n = length tl in
   if n = 0 then ()
   else
@@ -40,13 +40,18 @@ let rec lemma_thread_id_state_aux (tl: verifiable_log):
 
 let lemma_thread_id_state = lemma_thread_id_state_aux
 
-let lemma_requires_key_in_store 
-  (tl: verifiable_log) 
+let lemma_state_transition (tl: verifiable_log) (i: idx tl):
+  Lemma (state_at tl (i + 1) ==
+         t_verify_step (state_at tl i) (index tl i)) = 
+  ()
+
+let lemma_requires_key_in_store
+  (tl: verifiable_log)
   (i:idx tl{requires_key_in_store (index tl i)}):
-  Lemma (store_contains (store_idx tl i) (V.key_of (index tl i))) =
+  Lemma (store_contains (store_at tl i) (V.key_of (index tl i))) =
   lemma_verifiable_implies_prefix_verifiable tl (i + 1)
 
-let rec blum_add_seq_aux (tl: verifiable_log): 
+let rec blum_add_seq_aux (tl: verifiable_log):
   Tot (S.seq ms_hashfn_dom)
   (decreases (length tl)) =
   let n = length tl in
@@ -60,12 +65,20 @@ let rec blum_add_seq_aux (tl: verifiable_log):
 
 let blum_add_seq = blum_add_seq_aux
 
+let hadd_at (tl: verifiable_log) (i:nat{i <= length tl}): ms_hash_value =
+  Valid?.hadd (state_at tl i)
+
+let lemma_hadd_unchanged (tl: verifiable_log) (i: idx tl{not (is_blum_add (index tl i))}):
+  Lemma (hadd_at tl i == hadd_at tl (i + 1)) = 
+  lemma_state_transition tl i;
+  ()
+
 let rec lemma_hadd_correct_aux (tl: verifiable_log):
   Lemma (requires True)
         (ensures (hadd tl = ms_hashfn (blum_add_seq tl)))
-        (decreases (length tl)) = 
+        (decreases (length tl)) =
   let n = length tl in
-  if n = 0 then 
+  if n = 0 then
     lemma_hashfn_empty()
   else (
     let tl' = prefix tl (n - 1) in
@@ -73,24 +86,84 @@ let rec lemma_hadd_correct_aux (tl: verifiable_log):
     let e = index tl (n - 1) in
     let h' = hadd tl' in
     lemma_hadd_correct_aux tl';
-    if is_blum_add e then 
-      lemma_hashfn_app s' (blum_add_elem e)    
-    else ()
+    if is_blum_add e then lemma_hashfn_app s' (blum_add_elem e)      
+    else lemma_hadd_unchanged tl (n - 1)      
   )
 
-let lemma_hadd_correct = lemma_hadd_correct_aux 
+let lemma_hadd_correct = lemma_hadd_correct_aux
 
-let blum_evict_elem (tl: verifiable_log) (i:idx tl{is_evict_to_blum (index tl i)}): ms_hashfn_dom =  
-  admit()
+let blum_evict_elem (tl: verifiable_log) (i:idx tl{is_evict_to_blum (index tl i)}): ms_hashfn_dom =
+  let tli = prefix tl i in
+  let tli' = prefix tl (i + 1) in
+  let e = index tl i in
+  match e with
+  | EvictB k t -> 
+    let st = store_at tl i in
+    let v = stored_value st k in
+    MHDom (k,v) t (thread_id_of tl) 
+  | EvictBM k k' t -> 
+    let st = store_at tl i in
+    let v = stored_value st k in
+    MHDom (k,v) t (thread_id_of tl)   
 
-let blum_evict_seq (tl: verifiable_log): S.seq ms_hashfn_dom = admit()
+let rec blum_evict_seq_aux (tl: verifiable_log): 
+  Tot (S.seq ms_hashfn_dom)
+  (decreases (length tl)) = 
+  let n = length tl in
+  if n = 0 then S.empty #ms_hashfn_dom
+  else (
+    let tl' = prefix tl (n - 1) in
+    let s' = blum_evict_seq_aux tl' in
+    let e = index tl (n - 1) in
+    if is_evict_to_blum e then
+      SA.append1 s' (blum_evict_elem tl (n - 1))
+    else s'
+  )
+
+let blum_evict_seq (tl: verifiable_log): S.seq ms_hashfn_dom = 
+  blum_evict_seq_aux tl
+
+let hevict_at (tl: verifiable_log) (i:nat{i <= length tl}): ms_hash_value =
+  Valid?.hevict (state_at tl i)
+
+let lemma_hevict_unchanged (tl:verifiable_log) (i:idx tl{not (is_evict_to_blum (index tl i))}):
+  Lemma (hevict_at tl i = hevict_at tl (i + 1)) = ()
+
+let lemma_hevict_change (tl: verifiable_log) (i: idx tl{is_evict_to_blum (index tl i)}):
+  Lemma (hevict_at tl (i + 1) = ms_hashfn_upd (blum_evict_elem tl i) (hevict_at tl i)) = 
+  lemma_state_transition tl i;
+  lemma_thread_id_state (prefix tl i);  
+  ()
+
+let rec lemma_hevict_correct_aux (tl: verifiable_log):
+  Lemma (requires True)
+        (ensures (hevict tl = ms_hashfn (blum_evict_seq tl)))
+        (decreases (length tl)) = 
+  let n = length tl in
+  if n = 0 then 
+    lemma_hashfn_empty()
+  else (
+    let tl' = prefix tl (n - 1) in
+    let s' = blum_evict_seq tl' in
+    let e = index tl (n - 1) in
+    let h' = hevict tl' in
+    lemma_hevict_correct_aux tl';
+    if is_evict_to_blum e then (
+      lemma_hashfn_app s' (blum_evict_elem tl (n - 1));
+      lemma_hevict_change tl (n - 1)
+    )
+    else 
+      lemma_hevict_unchanged tl (n - 1)    
+  )
+
 
 let lemma_hevict_correct (tl: verifiable_log):
-  Lemma (hevict tl = ms_hashfn (blum_evict_seq tl)) = admit()
+  Lemma (hevict tl = ms_hashfn (blum_evict_seq tl)) = 
+  lemma_hevict_correct_aux tl
 
 (* all elements of tl's blum_evict_seq contain tid of tl *)
 let lemma_evict_elem_tid (tl: verifiable_log):
   Lemma (all (is_of_thread_id (thread_id_of tl)) (blum_evict_seq tl)) = admit()
-  
+
 let lemma_evict_elem_unique (tl: verifiable_log) (i1 i2: SA.seq_index (blum_evict_seq tl)):
   Lemma (i1 <> i2 ==> S.index (blum_evict_seq tl) i1 <> S.index (blum_evict_seq tl) i2) = admit()
